Functional sequential list spec

isabelle/List_Spec.thy
@@ -6,22 +6,20 @@ datatype 'oid list_op
   = InsertAfter 'oid
   | Remove 'oid
 
-definition insert_after :: "'oid \<Rightarrow> 'oid \<Rightarrow> ('oid \<rightharpoonup> 'oid) \<Rightarrow> ('oid \<rightharpoonup> 'oid)" where
-  "insert_after oid ref next \<equiv> (next(ref := Some oid))(oid := next ref)"
+fun insert_after :: "'oid \<Rightarrow> 'oid \<Rightarrow> 'oid list \<Rightarrow> 'oid list" where
+  "insert_after oid ref [] = []" |
+  "insert_after oid ref (x#xs) = (if x = ref then x#oid#xs else x # (insert_after oid ref xs))"
 
-definition remove :: "'oid \<Rightarrow> ('oid \<rightharpoonup> 'oid) \<Rightarrow> ('oid \<rightharpoonup> 'oid)" where
-  "remove ref next \<equiv>
-     if \<exists>p. next p = Some ref then
-       let p = THE p. next p = Some ref
-       in next(p := next ref)
-     else next"
+fun remove :: "'oid \<Rightarrow> 'oid list \<Rightarrow> 'oid list" where
+  "remove ref [] = []" |
+  "remove ref (x # xs) = (if x = ref then xs else x # (remove ref xs))"
 
-fun interp :: "('oid \<rightharpoonup> 'oid) \<Rightarrow> ('oid \<times> 'oid list_op) \<Rightarrow> ('oid \<rightharpoonup> 'oid)" where
-  "interp next (oid, InsertAfter ref) = insert_after oid ref next" |
-  "interp next (oid, Remove      ref) = remove ref next"
+fun interp :: "'oid list \<Rightarrow> ('oid \<times> 'oid list_op) \<Rightarrow> 'oid list" where
+  "interp list (oid, InsertAfter ref) = insert_after oid ref list" |
+  "interp list (oid, Remove      ref) = remove ref list"
 
-definition interp_list :: "('oid \<times> 'oid list_op) list \<Rightarrow> ('oid \<rightharpoonup> 'oid)" where
-  "interp_list ops \<equiv> foldl interp Map.empty ops"
+definition interp_list :: "('oid \<times> 'oid list_op) list \<Rightarrow> 'oid list" where
+  "interp_list ops \<equiv> foldl interp [] ops"
 
 fun oid_reference :: "'oid list_op \<Rightarrow> 'oid" where
   "oid_reference (InsertAfter ref) = ref" |
@@ -38,17 +36,16 @@ context list_spec begin
 definition op_set :: "('oid::{linorder} \<times> 'oid list_op) set" where
   "op_set \<equiv> set op_list"
 
-definition elems :: "('oid \<times> 'oid list_op) list" where
-  "elems \<equiv> filter (\<lambda>(_, oper). case oper of InsertAfter x \<Rightarrow> True | _ \<Rightarrow> False ) op_list"
-  
-definition next_elem :: "'oid \<rightharpoonup> 'oid" where
-  "next_elem \<equiv> interp_list op_list"
-  
-inductive next_elem_tc :: "'oid \<Rightarrow> 'oid \<Rightarrow> bool" (infix "\<sqsubset>" 50) where
-  next_elem_tcI1: "next_elem a = Some b \<Longrightarrow> a \<sqsubset> b " |
-  next_elem_tcI2: "a \<sqsubset> b \<Longrightarrow> next_elem b = Some c \<Longrightarrow> a \<sqsubset> c"
-  
-inductive_cases next_elem_tcE [elim]: "a \<sqsubset> b"
+definition insertions :: "('oid \<times> 'oid list_op) list" where
+  "insertions \<equiv> filter (\<lambda>(_, oper). case oper of InsertAfter x \<Rightarrow> True | _ \<Rightarrow> False ) op_list"
+
+definition the_list :: "'oid list" where
+  "the_list \<equiv> interp_list op_list"
+
+inductive list_order :: "'oid \<Rightarrow> 'oid \<Rightarrow> bool" (infix "\<sqsubset>" 50) where
+  "\<lbrakk>the_list = xs @ [x] @ ys @ [y] @ zs\<rbrakk> \<Longrightarrow> x \<sqsubset> y"
+
+inductive_cases list_order_elim [elim]: "x \<sqsubset> y"
 
 end
   
@@ -58,72 +55,236 @@ lemma list_spec_rm_last:
   using assms apply (clarsimp simp: list_spec_def)
   using sorted_append by blast
 
-lemma insert_next_1:
-  assumes "list_spec (op_list @ [(oid, InsertAfter ref)])"
-  shows "list_spec.next_elem (op_list @ [(oid, InsertAfter ref)]) ref = Some oid"
-  using assms apply(simp add: list_spec.next_elem_def interp_list_def insert_after_def)
-  using list_spec.ref_older by fastforce
+lemma insert_after_set:
+  assumes "ref \<in> set xs"
+  shows "set (insert_after oid ref xs) = set xs \<union> {oid}"
+  using assms apply (induct xs, simp)
+  by (case_tac "a=ref", simp_all add: insert_commute sup_commute)
 
-lemma insert_next_2:
-  assumes "list_spec (op_list @ [(oid, InsertAfter ref)])"
-  shows "list_spec.next_elem (op_list @ [(oid, InsertAfter ref)]) oid =
-         list_spec.next_elem op_list ref"
-  using assms apply(simp add: list_spec.next_elem_def interp_list_def insert_after_def)
-  by (metis interp_list_def list_spec.next_elem_def list_spec_rm_last)
+lemma insert_after_nonex:
+  assumes "ref \<notin> set xs"
+  shows "insert_after oid ref xs = xs"
+  using assms apply (induct xs, simp)
+  by (case_tac "a=ref", simp_all add: insert_commute sup_commute)
 
-lemma insert_next_3:
-  assumes "list_spec (op_list @ [(oid, InsertAfter ref)])"
-    and "x \<noteq> oid" and "x \<noteq> ref"
-  shows "list_spec.next_elem (op_list @ [(oid, InsertAfter ref)]) x =
-         list_spec.next_elem op_list x"
-  using assms apply(simp add: list_spec.next_elem_def interp_list_def insert_after_def)
-  by (metis interp_list_def list_spec.next_elem_def list_spec_rm_last)
+lemma list_greater_non_memb:
+  fixes oid :: "'oid::{linorder}"
+  assumes "\<forall>x \<in> set xs. x < oid"
+  shows "oid \<notin> set xs"
+  using assms by blast
 
-lemma unique_previous:
+lemma insert_after_distinct:
+  fixes oid :: "'oid::{linorder}"
+  assumes "distinct xs"
+    and "\<forall>x \<in> set xs. x < oid" and "ref < oid"
+  shows "distinct (insert_after oid ref xs)"
+  using assms apply (induct xs, simp)
+  apply(case_tac "a=ref")
+  apply clarsimp
+  apply(rule conjI)
+  apply(metis list.set_intros(1) list_greater_non_memb set_ConsD)
+  using list_greater_non_memb apply blast
+  apply(subgoal_tac "a \<noteq> oid")
+  apply(subgoal_tac "insert_after oid ref (a # xs) = a # insert_after oid ref xs")
+  apply(metis UnE distinct.simps(2) empty_iff insertE insert_after_nonex insert_after_set
+    list.set_intros(2))
+  apply auto
+  done
+
+lemma list_remove_set:
+  assumes "distinct xs"
+  shows "set (remove ref xs) = set xs - {ref}"
+  using assms apply (induct xs, simp)
+  by (case_tac "a=ref", auto)
+
+lemma list_remove_subset:
+  shows "set (remove ref xs) \<subseteq> set xs"
+  by (induct xs, auto)
+
+lemma remove_distinct:
+  assumes "distinct xs"
+  shows "distinct (remove ref xs)"
+  using assms apply (induct xs, simp)
+  apply(case_tac "a=ref", simp)
+  using list_remove_subset by fastforce
+
+lemma list_oid_subset:
   assumes "list_spec op_list"
-    and "list_spec.next_elem op_list p1 = Some x"
-    and "list_spec.next_elem op_list p2 = Some x"
-  shows "p1 = p2"
-  using assms apply(induct op_list rule: rev_induct)
-  apply(simp add: list_spec.next_elem_def interp_list_def)
+  shows "set (list_spec.the_list op_list) \<subseteq> set (map fst op_list)"
+  using assms apply (induct op_list rule: rev_induct)
+  apply(simp add: list_spec.the_list_def interp_list_def)
   apply(frule list_spec_rm_last, clarsimp)
   apply(case_tac b)
-  apply(case_tac "p1=x1")
+  apply(clarsimp simp add: list_spec.the_list_def interp_list_def)
+  apply(case_tac "x1 \<in> set (list_spec.the_list xs)")
+  apply(metis UnE empty_iff insert_after_set insert_iff interp_list_def list_spec.the_list_def subsetCE)
+  apply(simp add: contra_subsetD insert_after_nonex interp_list_def list_spec.the_list_def)
+  apply(clarsimp simp add: list_spec.the_list_def interp_list_def)
+  apply(subgoal_tac "x \<in> set (foldl interp [] xs)", blast)
+  apply(meson contra_subsetD list_remove_subset)
+  done
 
+lemma last_op_greatest:
+  assumes "list_spec (op_list @ [(oid, oper)])"
+  shows "\<forall>x \<in> set (map fst op_list). x < oid"
+  using assms apply(induct op_list, simp)
+  apply(subgoal_tac "sorted (map fst (op_list @ [(oid, oper)]))") prefer 2
+  using list_spec.sorted_oids sorted_Cons apply fastforce
+  apply(subgoal_tac "list_spec (op_list @ [(oid, oper)])") prefer 2
+  apply(simp add: list_spec_def, clarsimp)
+  apply(subgoal_tac "\<forall>x \<in> set (map fst op_list @ [oid]). a < x", simp)
+  apply(metis (no_types, lifting) distinct.simps(2) dual_order.strict_iff_order
+    list.map(1) list.simps(9) list_spec.distinct_oids list_spec.sorted_oids map_append
+    prod.sel(1) sorted_Cons)
+  done
 
-lemma remove_next_1:
-  assumes "list_spec (op_list @ [(oid, Remove ref)])"
-    and "list_spec.next_elem op_list prev = Some ref"
-  shows "list_spec.next_elem (op_list @ [(oid, Remove ref)]) prev =
-         list_spec.next_elem op_list ref"
-  using assms apply(simp add: list_spec.next_elem_def interp_list_def)
-  apply(subgoal_tac "\<exists>p. foldl interp Map.empty op_list p = Some ref") prefer 2
-  apply(metis interp_list_def list_spec.next_elem_def list_spec_rm_last)
-  apply(simp add: remove_def)
-  oops
-
-lemma next_elem_in_opset:
+lemma list_distinct:
   assumes "list_spec op_list"
-    and "list_spec.next_elem op_list a = Some b"
-  shows "{a, b} \<subseteq> set (map fst op_list) \<union> set (map (oid_reference \<circ> snd) op_list)"
-  using assms apply (induct op_list arbitrary: a b rule: rev_induct)
-  apply(simp add: list_spec.next_elem_def interp_list_def insert_after_def)
+  shows "distinct (list_spec.the_list op_list)"
+  using assms apply (induct op_list rule: rev_induct)
+  apply(simp add: list_spec.the_list_def interp_list_def)
   apply(frule list_spec_rm_last, clarsimp)
   apply(case_tac b, clarsimp)
-  apply(metis insert_next_1 insert_next_2 insert_next_3 option.sel)
+  apply(simp add: list_spec.the_list_def interp_list_def)
+  apply(rule insert_after_distinct, assumption)
+  apply(metis last_op_greatest interp_list_def list_oid_subset list_spec.the_list_def subset_code(1))
+  apply(simp add: list_spec_def)
+  apply(simp add: list_spec.the_list_def interp_list_def)
+  apply(simp add: remove_distinct)
+  done
 
+lemma suffix_eq_distinct_list:
+  assumes "ys@suf1 = xs"
+      and "ys@suf2 = xs"
+    shows "suf1 = suf2"
+using assms by(induction xs arbitrary: suf1 suf2 rule: rev_induct, simp) (metis append_eq_append_conv)
 
-lemma "list_spec.next_elem_tc A a b \<Longrightarrow> list_spec A \<Longrightarrow> a \<in> (fst ` set A)"
-  apply (erule list_spec.next_elem_tc.induct[rotated])
-    prefer 3
-    apply simp
-  prefer 2
-   apply force
-    using next_elem_in_opset
-  apply (force simp add: list_spec.next_elem_def interp_list_def insert_after_def)
-done
-    
-  
+lemma distinct_list_split:
+  assumes "distinct xs"
+    and "xs = xa @ x # ya"
+    and "xs = xb @ x # yb"
+  shows "xa = xb \<and> ya = yb"
+  using assms apply(induction xs arbitrary: xa xb x, simp)
+  apply(case_tac xa; case_tac xb; clarsimp)
+  done
+
+lemma list_order_trans:
+  assumes "list_spec op_list"
+    and "list_spec.list_order op_list x y"
+    and "list_spec.list_order op_list y z"
+  shows "list_spec.list_order op_list x z"
+  using assms apply -
+  apply(subgoal_tac "\<exists>ws xs ys zs. list_spec.the_list op_list = ws@[x]@xs@[y]@ys@[z]@zs")
+  apply(metis append.assoc list_spec.list_order.intros)
+  apply(erule_tac x=x and y=y in list_spec.list_order_elim, assumption)
+  using assms(1) apply -
+  apply(erule_tac x=y and y=z in list_spec.list_order_elim, assumption)
+  apply(subgoal_tac "distinct (list_spec.the_list op_list)") prefer 2
+  using assms(1) list_distinct apply blast
+  apply(subgoal_tac "zs = ysa @ z # zsa") prefer 2
+  apply(frule_tac xa="xs @ x # ys" and xb=xsa and x=y and ya=zs
+    and yb="ysa @ z # zsa" in distinct_list_split, simp, simp, simp)
+  apply(rule_tac x=xs in exI, rule_tac x=ys in exI)
+  apply(rule_tac x=ysa in exI, rule_tac x=zsa in exI, simp)
+  done
+
+lemma insert_somewhere:
+  assumes "ref \<in> set list"
+  shows "\<exists>xs ys. list = xs@ys \<and> insert_after oid ref list = xs @ oid # ys"
+  using assms apply(induction list, simp)
+  apply(case_tac "a=ref")
+  apply(rule_tac x="[ref]" in exI, rule_tac x=list in exI, simp)
+  apply(subgoal_tac "ref \<in> set list", simp) prefer 2 apply simp
+  apply(erule exE)+
+  apply(rule_tac x="a#xs" in exI, rule_tac x=ys in exI, force)
+  done
+
+lemma insert_first_part:
+  assumes "ref \<in> set xs"
+  shows "insert_after oid ref (xs @ ys) = (insert_after oid ref xs) @ ys"
+  using assms
+  apply(induction ys rule: rev_induct, simp, simp)
+  apply(induction xs, simp)
+  apply(case_tac "a=ref", simp_all)
+  done
+
+lemma insert_second_part:
+  assumes "ref \<notin> set xs"
+    and "ref \<in> set ys"
+  shows "insert_after oid ref (xs @ ys) = xs @ (insert_after oid ref ys)"
+  using assms
+  apply(induction xs, simp, simp)
+  apply(subgoal_tac "a \<noteq> ref", blast+)
+  done
+
+lemma insert_twice:
+  assumes "list_spec (before @ (x1, InsertAfter r1) # after @ [(x2, InsertAfter r2)])"
+    and   "list_spec (before @                        after @ [(x2, InsertAfter r2)])"
+    and "list_spec.the_list (before @                        after) = xs @      zs"
+    and "list_spec.the_list (before @ (x1, InsertAfter r1) # after) = xs @ ys @ zs"
+  shows "\<exists>xsa ysa zsa.
+    list_spec.the_list (before @                        after @ [(x2, InsertAfter r2)]) = xsa @       zsa \<and>
+    list_spec.the_list (before @ (x1, InsertAfter r1) # after @ [(x2, InsertAfter r2)]) = xsa @ ysa @ zsa"
+  using assms apply -
+  apply(subgoal_tac "list_spec (before @ after)") prefer 2
+  using list_spec_rm_last apply force
+  apply(subgoal_tac "list_spec (before @ (x1, InsertAfter r1) # after)") prefer 2
+  using list_spec_rm_last apply force
+  apply(simp add: list_spec.the_list_def interp_list_def)
+  apply(case_tac "r2 \<in> set xs")
+  using insert_first_part apply fastforce
+  apply(case_tac "r2 \<in> set ys")
+  apply(rule_tac x=xs in exI)
+  apply(rule_tac x="insert_after x2 r2 ys" in exI)
+  apply(rule_tac x=zs in exI)
+  apply(rule conjI)
+  apply(subgoal_tac "r2 \<notin> set zs")
+  apply(simp add: insert_after_nonex)
+  using assms(4) distinct_append list.simps(15) list_distinct apply force
+  apply(simp add: insert_first_part insert_second_part)
+  apply(case_tac "r2 \<in> set zs")
+  apply(rule_tac x=xs in exI)
+  apply(rule_tac x=ys in exI)
+  apply(rule_tac x="insert_after x2 r2 zs" in exI)
+  apply(simp add: insert_second_part)
+  apply(metis UnE insert_after_nonex set_append)
+  done
+
+lemma insert_preserves_order:
+  assumes "list_spec op_list" and "list_spec rest"
+    and "rest = before @ after"
+    and "op_list = before @ (oid, InsertAfter ref) # after"
+  shows "\<exists>xs ys zs. list_spec.the_list rest    = xs @      zs \<and>
+                    list_spec.the_list op_list = xs @ ys @ zs"
+  using assms
+  apply(induction after arbitrary: rest op_list rule: rev_induct)
+  apply(case_tac "ref \<in> set (list_spec.the_list before)")
+  apply(subgoal_tac "\<exists>xs zs. list_spec.the_list rest = xs@zs \<and>
+                             list_spec.the_list op_list = xs@[oid]@zs", blast)
+  apply(simp add: list_spec.the_list_def interp_list_def insert_somewhere)
+  apply(subgoal_tac "list_spec.the_list op_list = list_spec.the_list rest", force)
+  apply(simp add: list_spec.the_list_def interp_list_def insert_after_nonex)
+  apply(erule_tac x="before @ xs" in meta_allE)
+  apply(erule_tac x="before @ (oid, InsertAfter ref) # xs" in meta_allE)
+  apply(subgoal_tac "list_spec (before @ xs)") prefer 2
+  apply(metis append_assoc list_spec_rm_last)
+  apply(subgoal_tac "list_spec (before @ (oid, InsertAfter ref) # xs)") prefer 2
+  apply(metis append_butlast_last_id append_is_Nil_conv butlast.simps(2) butlast_append
+    butlast_snoc list.distinct(1) list_spec_rm_last)
+  apply clarsimp
+  apply(case_tac b, simp add: insert_twice)
+  apply clarsimp
+  oops
+
+lemma
+  assumes "list_spec A" and "list_spec B"
+    and "set A \<subseteq> set B"
+    and "A = list_spec.insertions A"
+    and "B = list_spec.insertions B"
+    and "list_spec.list_order A x y"
+  shows "list_spec.list_order B x y"
+  oops
+
 lemma "list_spec.next_elem_tc A a b \<Longrightarrow> list_spec A \<Longrightarrow> list_spec (A@[(oid, InsertAfter ref)]) \<Longrightarrow> list_spec.next_elem_tc (A@[(oid, InsertAfter ref)]) a b" 
   apply (erule list_spec.next_elem_tc.cases)
     apply assumption
